execution/theories/Generators.v
@@ -5,12 +5,13 @@ From ExtLib.Structures Require Import Functor Applicative.
 From ConCert Require Import Blockchain.
 From ConCert Require Import LocalBlockchain.
 From ConCert Require Import Serializable.
-
+From ConCert Require Import BoundedN.
 (* For monad notations *)
 Require Export ExtLib.Structures.Monads.
 Export MonadNotation. Open Scope monad_scope.
 
 From Coq Require Import List.
+From Coq Require Import Strings.BinaryString.
 Import ListNotations.
 
 (* Module DoNotation.
@@ -33,16 +34,15 @@ Instance showAmount : Show Amount :=
 
 Instance genAmountSized : GenSized Amount :=
   {|
-    arbitrarySized := @arbitrarySized Z genZSized 
+    arbitrarySized := @arbitrarySized Z _ 
   |}.
 
 Instance shrinkAmount : Shrink Amount := 
   {|
-    shrink := @shrink Z shrinkZ
+    shrink := @shrink Z _
   |}.
 
-(* making show and generator instances for the Chain type *)
-
+  
 (* dummy implementation for now *)
 Definition empty_str : string := "".
 Definition sep : string := ", ".
@@ -72,21 +72,7 @@ Instance showChain (BaseTypes : ChainBase) : Show (@Chain BaseTypes) :=
 
 Close Scope string_scope.
 
-Instance genChainSized (BaseTypes : ChainBase) : GenSized (@Chain BaseTypes) :=
-  {|
-    arbitrarySized n := 
-      returnGen (build_chain n n n (fun (a : Blockchain.Address) => Z.of_nat n))
-  |}.
 
-Definition a := vectorOf 2 (returnGen 10).
-Print a.
-Sample a.
-
-(* For now, shrinking does nothing *)
-Instance shrinkChain (BaseTypes : ChainBase) : Shrink (@Chain BaseTypes) :=
-  {|
-    shrink c := cons c nil
-  |}.
 
 Fixpoint mkMapFromList {B : Type}
                        (address_eqb : Address -> Address -> bool)
@@ -110,8 +96,8 @@ Definition mkMapFromListGen {B : Type}
                           : G (Address -> B) :=
   listA <- genListA ;; mkMapFromList address_eqb genB listA.
 
-
-
+(* Makes a generator for BlockChains, given generators for the necessary types: Address, Setup, Msg, State, SerializedValue. 
+   Ensures that all address usages are consistent with the generated address mapping. *)
 Definition mkChainGen {Setup Msg State : Type}
                         (baseGens : @BaseGens Setup Msg State) (BaseTypes : ChainBase)
                         : nat -> G (@Chain BaseTypes)  := 
@@ -125,40 +111,94 @@ Definition mkChainGen {Setup Msg State : Type}
     mp         <- mkMapFromListGen addr_eqb (sized arbitrarySized) addr_list_gen ;; 
     returnGen (build_chain ch_height cur_slot n (fun (a : Blockchain.Address) => Z.of_nat n)).
 
+  (* For now, shrinking does nothing *)
+Instance shrinkChain (BaseTypes : ChainBase) : Shrink (@Chain BaseTypes) :=
+  {|
+    shrink c := cons c nil
+  |}.
+
 
 
 Module LocalBlockchainGens.
-Require Import LocalBlockchain.
-Require Import BoundedN.
+
+Import BoundedN.Stdpp.
+Global Opaque Address. 
 
 Print LocalChainBase.
 
-Global Opaque Address. 
-
 Definition b10 : Address := BoundedN.of_Z_const AddrSize 10.
-Print N.to_nat.
-(* First we define an auxilliary generator for Addresses*)
-Definition genAddress : G (BoundedN.BoundedN AddrSize) :=
-  n <- arbitrarySized (N.to_nat AddrSize) ;;
-  let 
-    boundedNOpt : option (BoundedN.BoundedN AddrSize) := @BoundedN.of_nat AddrSize n
-  in returnGen match boundedNOpt with
-  | Some b => b
-  (* The None case should never happen since 'arbitrarySized' on AddrSize already ensures that
-     n <= AddrSized. *)
-  | None => BoundedN.of_Z_const AddrSize 0
-  end.
+Definition b9 : option (BoundedN.BoundedN AddrSize) := @BoundedN.of_nat AddrSize 9.
+
+
+(* Show instances *)
+Open Scope string_scope.
+(* For a more memory efficient method, use BinaryString.of_N instead (but this prints numbers in binary notation, ie. eg. 0b0010) *)
+Instance showN : Show N :=
+  {|
+    show n := show (N.to_nat n)   
+  |}.
+
+
+(* We dont show the bound because it may be a very large number which, when converted to nat and then to string, gives a memory overflow. *)
+Instance showBoundedN {bound : N} `{Show N} : Show (BoundedN.BoundedN bound) :=
+  {|
+    show bn := match bn with | BoundedN.bounded n _ => show n ++ "%" ++ show bound end  
+  |}.
+ 
+
+Instance showBoundedNAddrSize : Show (BoundedN.BoundedN AddrSize) :=
+  {|
+    show := @show (BoundedN.BoundedN AddrSize) showBoundedN
+  |}.
+
+Instance showAddress : Show Address :=
+  {|
+    show := @show (BoundedN.BoundedN AddrSize) showBoundedN
+  |}.
+
+
+
+Close Scope string_scope.
+
+(* Generators *)
+Definition genZ : G Z := arbitrary.	
+
+
+Derive Show for positive.
+Derive Arbitrary for positive.
+Derive GenSized for positive.
+
+(* Although the type is G (option ...) it will never generate None values *)
+Definition genBoundedNOpt (bound : N): G (option (BoundedN.BoundedN bound)) :=
+  n <- arbitrarySized (N.to_nat bound) ;; (* we exploit that arbitrarySized n on nats automatically bounds the value by <= n *)
+  returnGen (@decode_bounded bound (Pos.of_nat n)).
+
+
+Definition genBoundedN : G (BoundedN.BoundedN AddrSize) :=
+  bn <- genBoundedNOpt AddrSize ;;
+  returnGen match bn with
+    | Some b => b
+    (** The None case should never happen since 'arbitrarySized' on AddrSize already ensures that
+        n <= AddrSized. **)
+    | None => BoundedN.of_Z_const AddrSize 0
+  end. 
+
+Definition genAddress : G Address := genBoundedN.
 
 
 
 End LocalBlockchainGens.
 
 
+Import LocalBlockchainGens.
+
+Sample genAddress.
+
 
 Sample (@arbitrarySized Chain (genChainSized LocalChainBase) 2).
 
 
-Sample (@arbitrarySized Amount genAmountSized 2).
+Sample (@arbitrarySized Amount _ 2).
 
 Open Scope nat_scope.
 Definition n_is_zero_nat (n : nat) := n =? 0.
